WPDS/WExInstances.thy
@@ -4,19 +4,12 @@ begin
 
 (* Define rules of PDS, and the two P-automata *)
 
-definition pds_rules :: "(ctr_loc, label) rule set" where
-  "pds_rules = {
-  ((p1, B), (p1, push A B)),
-  ((p1, A), (p2, swap B)),
-  ((p2, A), (p3, pop)),
-  ((p3, B), (p2, swap A))}"
-definition W :: "(ctr_loc, label) rule \<Rightarrow> nat_inf" where
-  "W rule = (K$ infinity)
-    (((p1, B), (p1, push A B)) $:= fin 1)
-    (((p1, A), (p2, swap B))   $:= fin 2)
-    (((p2, A), (p3, pop))      $:= fin 3)
-    (((p3, B), (p2, swap A))   $:= fin 4) $ rule"
-
+definition pds_rules :: "(ctr_loc, label, nat_inf) w_rule list" where
+  "pds_rules = [
+  ((p1, B), fin 1, (p1, push A B)),
+  ((p1, A), fin 2, (p2, swap B)),
+  ((p2, A), fin 3, (p3, pop)),
+  ((p3, B), fin 4, (p2, swap A))]"
 definition initial_automaton :: "((ctr_loc, state) WPDS.state, label) transition set" where
   "initial_automaton = {
   ((Init p1, B, Noninit qf)),
@@ -35,16 +28,10 @@ definition "final_finals = {Noninit q2}"
 (* Query specific part END *)
 
 
-
-definition pds_rules_900 :: "(ctr_loc, label) rule set" where
-  "pds_rules_900 = {
-  ((p0, A), (p0, push A A)),
-  ((p1, B), (p0, push A B))}"
-definition pds_rules_900_W :: "(ctr_loc, label) rule => nat_inf" where
-  "pds_rules_900_W rule = (K$ infinity)
-  (((p0, A), (p0, push A A)) $:= fin 2)
-  (((p1, B), (p0, push A B)) $:= fin 2)
- $ rule"
+definition pds_rules_900 :: "(ctr_loc, label, nat_inf) w_rule list" where
+  "pds_rules_900 = [
+  ((p0, A), fin 2, (p0, push A A)),
+  ((p1, B), fin 2, (p0, push A B))]"
 definition initial_100_automaton :: "((ctr_loc, state) WPDS.state, label) transition set" where
   "initial_100_automaton = {
   ((Init p0, A, Noninit q2)),
@@ -56,9 +43,9 @@ definition final_100_automaton :: "((ctr_loc, state) WPDS.state, label) transiti
   ((Noninit q2, B, Noninit q2))}"
 definition final_100_finals where "final_100_finals = {}"
 
-value "run_WPDS_reach pds_rules_900 pds_rules_900_W initial_100_automaton final_100_automaton initial_100_finals final_100_finals"
+value "run_WPDS_reach pds_rules_900 initial_100_automaton final_100_automaton initial_100_finals final_100_finals"
 
-definition "ex3 == run_WPDS_reach pds_rules W initial_automaton final_automaton initial_finals final_finals"
+definition "ex3 == run_WPDS_reach pds_rules initial_automaton final_automaton initial_finals final_finals"
 
 lemma
   "ex3 = Some (fin 3)"
